\documentclass[10pt]{article}
\usepackage[utf8]{inputenc}
\usepackage{amsmath}
\usepackage{amssymb}
\usepackage{graphicx}
\usepackage{geometry}
\usepackage{enumitem}
\usepackage{multicol}
\usepackage{ifthen}
\geometry{a4paper, margin=1in}

\pagestyle{empty} % Completely remove page numbers

\title{\vspace{-1.5cm}\Large\textbf{University of Nebraska-Lincoln}\\[0.2cm]
\Large\textbf{Digital Signal Processing: Quiz 1}} % Add institution and make title larger
\date{\vspace{-0.5cm}\small\textbf{August 29, 2025}} % Format the date professionally

\newboolean{showresults}
\setboolean{showresults}{false}

\begin{document}

\maketitle

\noindent\textbf{Name:} \underline{\hspace{10cm}} \hfill \textbf{Total Points: 10}


\vspace{0.5cm}

\begin{enumerate}
    \item \textbf{(10 points)} Consider the frequency response
    \[
    H(e^{j\omega}) = \frac{1 + e^{-j\omega}}{3 - 2e^{-j\omega}}
    \]
     Find the \textbf{real part} of $H(e^{j\omega})$ as a function of $\omega$. \textbf{Note:} don't leave any $j$'s, $i$'s, $\sqrt{-1}$'s, etc. \\
    
    
    % \vspace{8cm}

    \ifthenelse{\boolean{showresults}}{
        \textbf{Solution:}
    
            First, express all terms in terms of sines and cosines:
            \[
            e^{-j\omega} = \cos\omega - j\sin\omega
            \]
            \[
            1 + e^{-j\omega} = 1 + \cos\omega - j\sin\omega
            \]
            \[
            3 - 2e^{-j\omega} = 3 - 2\cos\omega + j2\sin\omega
            \]
            Let $A = 1 + \cos\omega$, $B = -\sin\omega$, $C = 3 - 2\cos\omega$, $D = 2\sin\omega$,
            so
            \[
            H(e^{j\omega}) = \frac{A + jB}{C + jD}
            \]
            Multiply numerator and denominator by the complex conjugate of the denominator:
            \[
            (C - jD)
            \]
            \[
            H(e^{j\omega}) = \frac{(A + jB)(C - jD)}{(C + jD)(C - jD)}
            \]
            \[
            = \frac{AC + BD + j(BC - AD)}{C^2 + D^2}
            \]
            The real part is:
            \[
            \operatorname{Re}\left\{ H(e^{j\omega}) \right\} = \frac{AC + BD}{C^2 + D^2}
            \]
            Substitute back:
            \[
            AC = (1 + \cos\omega)(3 - 2\cos\omega) = 3 + 3\cos\omega - 2\cos\omega - 2\cos^2\omega = 3 + \cos\omega - 2\cos^2\omega
            \]
            \[
            BD = (-\sin\omega)(2\sin\omega) = -2\sin^2\omega
            \]
            \[
            AC + BD = 3 + \cos\omega - 2\cos^2\omega - 2\sin^2\omega
            \]
            Recall that $\sin^2\omega + \cos^2\omega = 1$, so:
            \[
            -2\cos^2\omega - 2\sin^2\omega = -2(\cos^2\omega + \sin^2\omega) = -2
            \]
            \[
            AC + BD = 3 + \cos\omega - 2 = 1 + \cos\omega
            \]
            The denominator:
            \[
            C^2 + D^2 = (3 - 2\cos\omega)^2 + [2\sin\omega]^2 = 9 -12\cos\omega + 4\cos^2\omega + 4\sin^2\omega
            \]
            \[
            = 9 - 12\cos\omega + 4(\cos^2\omega + \sin^2\omega)
            \]
            \[
            = 9 - 12\cos\omega + 4(1) = 13 - 12\cos\omega
            \]
            Therefore,
            \[
            \boxed{
            \operatorname{Re}\left\{ H(e^{j\omega}) \right\} = \frac{1 + \cos\omega}{13 - 12\cos\omega}
            }
            \]
        
    }{}
    \end{enumerate}

\end{document}